add ability to handle context

proofs/program.v
@@ -28,50 +28,62 @@ Inductive prog :=
   (* add while/for/try/def *)
 .
 
-Inductive exec_p : environment -> prog -> environment -> list effect -> Prop :=
+Inductive continuation :=
+  | normal : continuation
+  | break : continuation
+  | continue : continuation
+  | returns : value -> continuation
+.
+
+Inductive exec_p : environment -> prog -> environment -> list effect -> continuation -> Prop :=
   | exec_p_e
     : forall env_1 env_2 effs e,
-      (exists x, exec_e env_1 e x effs) -> equal_env env_1 env_2 -> exec_p env_1 (prog_e e) env_2 effs
+      (exists x, exec_e env_1 e x effs) -> equal_env env_1 env_2 -> exec_p env_1 (prog_e e) env_2 effs normal
   | exec_p_a
     : forall env_1 env_2 effs v e,
-      (exists x, exec_e env_1 e x effs /\ env_2 = cons (v, x) env_1) -> exec_p env_1 (prog_a v e) env_2 effs
-  | exec_p_s
-    : forall env_1 env_2 effs p_1 p_2,
+      (exists x, exec_e env_1 e x effs /\ env_2 = cons (v, x) env_1) -> exec_p env_1 (prog_a v e) env_2 effs normal
+  | exec_p_s_normal
+    : forall env_1 env_2 effs p_1 p_2 c,
       (exists env_inter eff_1 eff_2,
-        exec_p env_1 p_1 env_inter eff_1 /\ exec_p env_inter p_2 env_2 eff_2 /\ app eff_1 eff_2 = effs
-      ) -> exec_p env_1 (prog_s p_1 p_2) env_2 effs
+        exec_p env_1 p_1 env_inter eff_1 normal /\ exec_p env_inter p_2 env_2 eff_2 c /\ app eff_1 eff_2 = effs
+      ) -> exec_p env_1 (prog_s p_1 p_2) env_2 effs c
+  (*| exec_p_s_abnormal
+    : forall env_1 env_2 effs p_1 p_2 c,
+      exec_p env_1 p_1 env_2 effs c /\ c <> normal
+       -> exec_p env_1 (prog_s p_1 p_2) env_2 effs c*)
   | exec_p_i
-    : forall env_1 env_2 effs cond p_1 p_2,
+    : forall env_1 env_2 effs cond p_1 p_2 c,
       (exists x eff_1 eff_2,
-        exec_e env_1 cond x eff_1 /\ exec_p env_1 (if truthy x then p_1 else p_2) env_2 eff_2 /\ app eff_1 eff_2 = effs
-      ) -> exec_p env_1 (prog_i cond p_1 p_2) env_2 effs
+        exec_e env_1 cond x eff_1 /\ exec_p env_1 (if truthy x then p_1 else p_2) env_2 eff_2 c /\ app eff_1 eff_2 = effs
+      ) -> exec_p env_1 (prog_i cond p_1 p_2) env_2 effs c
 .
 
 Hypothesis exec_e_deterministic : forall {env e x_a effs_a x_b effs_b},
   exec_e env e x_a effs_a -> exec_e env e x_b effs_b -> x_a = x_b /\ effs_a = effs_b.
 
-Theorem exec_p_deterministic : forall p env_1 env_2a effs_a env_2b effs_b,
-  exec_p env_1 p env_2a effs_a -> exec_p env_1 p env_2b effs_b -> equal_env env_2a env_2b /\ effs_a = effs_b.
+Theorem exec_p_deterministic : forall {p env_1 env_2a effs_a env_2b effs_b c_a c_b},
+  exec_p env_1 p env_2a effs_a c_a -> exec_p env_1 p env_2b effs_b c_b -> equal_env env_2a env_2b /\ effs_a = effs_b /\ c_a = c_b.
 
   induction p; intros; inversion H; inversion H0; subst.
   all: repeat match goal with
     | [H: exists _, _ |- _] => destruct H
     | [H: _ /\ _ |- _] => destruct H
     end.
-  all: try match goal with
-    | [H1: exec_e _ _ _ _, H2: exec_e _ _ _ _ |- _] => destruct (exec_e_deterministic H2 H1)
+  all: repeat match goal with
+    | [H1: exec_e _ _ _ _, H2: exec_e _ _ _ _ |- _] => destruct (exec_e_deterministic H2 H1); clear H1 H2
     end.
   all: unfold equal_env in *.
   all: subst.
-  all: try solve [split; auto].
-  - destruct (IHp1 _ _ _ _ _ H2 H1); subst.
-    destruct (IHp2 _ _ _ _ _ H5 H3); subst.
-    split; auto.
-  - destruct (truthy x2); simpl in *.
-    destruct (IHp1 _ _ _ _ _ H3 H5).
-    subst; split; auto.
-    destruct (IHp2 _ _ _ _ _ H3 H5).
-    subst; split; auto.
+  4: destruct (truthy x2).
+  all: repeat match goal with
+     | [
+      IH : forall _ _ _ _ _ _ _, exec_p _ ?p _ _ _ -> _,
+      HA : exec_p _ ?p _ _ _,
+      HB : exec_p _ ?p _ _ _
+     |- _] => 
+        destruct (IH _ _ _ _ _ _ _ HA HB) as [? [? ?]]; clear IH; subst
+   end.
+  all: try solve [subst; repeat split; auto].
 Qed.
 
 End programs.
